lawful -> constant

Clean/Circuit/LoopsForAll.lean
@@ -11,74 +11,74 @@ lemma Vector.forM_toList (xs : Vector α n) {m : Type → Type} [Monad m] (body 
 
 namespace Circuit
 
-lemma forAll_flatten (xs : Vector α m) {circuit : α → Circuit F β} (lawful : ConstantCircuits circuit)
+lemma forAll_flatten (xs : Vector α m) {circuit : α → Circuit F β} (constant : ConstantCircuits circuit)
   {prop : Operations.Condition F} :
-  Operations.forAll n prop (List.ofFn fun (i : Fin m) => (circuit xs[i.val]).operations (n + i * lawful.local_length)).flatten
-    ↔ ∀ (i : Fin m), (circuit xs[i.val]).forAll prop (n + i * lawful.local_length) := by
+  Operations.forAll n prop (List.ofFn fun (i : Fin m) => (circuit xs[i.val]).operations (n + i * constant.local_length)).flatten
+    ↔ ∀ (i : Fin m), (circuit xs[i.val]).forAll prop (n + i * constant.local_length) := by
   induction m generalizing n
   case zero => simp [Operations.forAll]
   case succ m ih =>
     rw [List.ofFn_succ, List.flatten_cons, Operations.forAll_append, Fin.forall_fin_succ, Circuit.forAll_def]
     simp only [Fin.val_zero, zero_mul, add_zero, Fin.val_succ]
-    specialize ih (n := n + lawful.local_length) (xs := xs.drop 1)
+    specialize ih (n := n + constant.local_length) (xs := xs.drop 1)
     simp only [Vector.drop_eq_cast_extract, Nat.add_one_sub_one, Vector.getElem_cast,
       Vector.getElem_extract] at ih
-    have : ((circuit xs[0]).operations n).local_length + n = n + lawful.local_length := by
-      rw [←lawful.local_length_eq (xs[0]) n]; ac_rfl
+    have : ((circuit xs[0]).operations n).local_length + n = n + constant.local_length := by
+      rw [←constant.local_length_eq (xs[0]) n]; ac_rfl
     rw [this]
     ring_nf at ih ⊢
     rw [ih]
 
 namespace ForM
-variable {circuit : α → Circuit F Unit} (xs : Vector α m) (lawful : ConstantCircuits circuit) (n : ℕ)
+variable {circuit : α → Circuit F Unit} (xs : Vector α m) (constant : ConstantCircuits circuit) (n : ℕ)
 
-theorem local_length_eq : (xs.forM circuit).local_length n = m * lawful.local_length := by
-  set k := lawful.local_length
+theorem local_length_eq : (xs.forM circuit).local_length n = m * constant.local_length := by
+  set k := constant.local_length
   induction xs using Vector.induct generalizing n
   case nil => ac_rfl
   case cons x xs ih =>
     rw [Vector.forM_toList, Vector.cons, List.forM_cons, ←Vector.forM_toList,
-      bind_local_length_eq, ih, lawful.local_length_eq]
+      bind_local_length_eq, ih, constant.local_length_eq]
     ring
 
 theorem output_eq : (xs.forM circuit).output n = () := rfl
 
 theorem operations_eq :
   (xs.forM circuit).operations n =
-    (List.ofFn fun (i : Fin m) => (circuit xs[i.val]).operations (n + i * lawful.local_length)).flatten := by
+    (List.ofFn fun (i : Fin m) => (circuit xs[i.val]).operations (n + i * constant.local_length)).flatten := by
   induction xs using Vector.induct generalizing n
   case nil => rfl
   case cons x xs ih =>
     rw [Vector.forM_toList, Vector.cons, List.forM_cons, ←Vector.forM_toList,
-      bind_operations_eq, ih, lawful.local_length_eq, List.ofFn_succ, List.flatten_cons]
+      bind_operations_eq, ih, constant.local_length_eq, List.ofFn_succ, List.flatten_cons]
     simp only [Vector.getElem_mk, List.getElem_toArray, Fin.val_zero, Fin.val_succ,
       List.getElem_zero, List.getElem_cons_succ, List.head_cons, Array.getElem_toList, Vector.getElem_toArray]
     ring_nf
 
 theorem forAll_iff {prop : Operations.Condition F} :
   (xs.forM circuit).forAll prop n ↔
-    ∀ (i : Fin m), (circuit xs[i.val]).forAll prop (n + i*lawful.local_length) := by
+    ∀ (i : Fin m), (circuit xs[i.val]).forAll prop (n + i*constant.local_length) := by
   rw [forAll_def, operations_eq, forAll_flatten]
 end ForM
 
 def forEach {m : ℕ} (xs : Vector α m) [Inhabited α] (body : α → Circuit F Unit)
-    (_lawful : ConstantCircuits body := by infer_constant_circuits) : Circuit F Unit :=
+    (_constant : ConstantCircuits body := by infer_constant_circuits) : Circuit F Unit :=
   xs.forM body
 
 section forEach
 variable {env : Environment F} {m n : ℕ} [Inhabited α] {xs : Vector α m}
-  {body : α → Circuit F Unit} {lawful : ConstantCircuits body} {prop : Operations.Condition F}
+  {body : α → Circuit F Unit} {constant : ConstantCircuits body} {prop : Operations.Condition F}
 
 @[circuit_norm ↓]
 lemma forEach.soundness :
-  constraints_hold.soundness env ((forEach xs body lawful).operations n) ↔
+  constraints_hold.soundness env ((forEach xs body constant).operations n) ↔
     ∀ i : Fin m, constraints_hold.soundness env (body xs[i.val] |>.operations (n + i*(body default).local_length)) := by
   simp only [forEach, constraints_hold.soundness_iff_forAll']
   rw [ForM.forAll_iff, ConstantCircuits.local_length_eq]
 
 /-- variant of `forEach.soundness`, for when the constraints don't depend on the input offset -/
 lemma forEach.soundness' :
-  constraints_hold.soundness env (forEach xs body lawful |>.operations n) →
+  constraints_hold.soundness env (forEach xs body constant |>.operations n) →
     ∀ x ∈ xs, ∃ k : ℕ, constraints_hold.soundness env (body x |>.operations k) := by
   simp only [forEach, constraints_hold.soundness_iff_forAll', ForM.forAll_iff]
   intro h x hx
@@ -87,32 +87,32 @@ lemma forEach.soundness' :
 
 @[circuit_norm ↓]
 lemma forEach.completeness :
-  constraints_hold.completeness env ((forEach xs body lawful).operations n) ↔
+  constraints_hold.completeness env ((forEach xs body constant).operations n) ↔
     ∀ i : Fin m, constraints_hold.completeness env (body xs[i.val] |>.operations (n + i*(body default).local_length)) := by
   simp only [forEach, constraints_hold.completeness_iff_forAll']
   rw [ForM.forAll_iff, ConstantCircuits.local_length_eq]
 
 @[circuit_norm ↓]
 lemma forEach.uses_local_witnesses :
-  env.uses_local_witnesses_completeness n ((forEach xs body lawful).operations n) ↔
+  env.uses_local_witnesses_completeness n ((forEach xs body constant).operations n) ↔
     ∀ i : Fin m, env.uses_local_witnesses_completeness (n + i*(body default).local_length) (body xs[i.val] |>.operations (n + i*(body default).local_length)) := by
   simp only [forEach, env.uses_local_witnesses_completeness_iff_forAll, ←forAll_def]
   rw [ForM.forAll_iff, ConstantCircuits.local_length_eq]
 
 @[circuit_norm ↓]
 lemma forEach.forAll :
-  Operations.forAll n prop ((forEach xs body lawful).operations n) ↔
+  Operations.forAll n prop ((forEach xs body constant).operations n) ↔
     ∀ i : Fin m, (body xs[i.val] |>.forAll prop (n + i*(body default).local_length)) := by
   simp only [forEach, ←forAll_def]
   rw [ForM.forAll_iff, ConstantCircuits.local_length_eq]
 
 @[circuit_norm ↓]
 lemma forEach.local_length_eq :
-    (forEach xs body lawful).local_length n = m * (body default).local_length := by
-  rw [forEach, ForM.local_length_eq, lawful.local_length_eq]
+    (forEach xs body constant).local_length n = m * (body default).local_length := by
+  rw [forEach, ForM.local_length_eq, constant.local_length_eq]
 
 @[circuit_norm ↓]
 lemma forEach.output_eq :
-  (forEach xs body lawful).output n = () := rfl
+  (forEach xs body constant).output n = () := rfl
 
 end forEach
